HybridVerifVecs/hs_vc_spartan.thy
@@ -11,28 +11,30 @@ type_synonym 'a pred = "'a \<Rightarrow> bool"
 no_notation Transitive_Closure.rtrancl ("(_\<^sup>*)" [1000] 999)
 
 notation Union ("\<mu>")
+     and g_orbital ("(1x\<acute>=_ & _ on _ _ @ _)")
 
-definition fbox :: "('a \<Rightarrow> 'b set) \<Rightarrow> 'b pred \<Rightarrow> 'a pred"
-  where "fbox F P = (\<lambda>s. (\<forall>s'. s' \<in> F s \<longrightarrow> P s'))"
+abbreviation "skip \<equiv> (\<lambda>s. {s})"
 
 section \<open>Verification of regular programs\<close>
 
 text \<open>First we add lemmas for computation of weakest liberal preconditions (wlps).\<close>
 
-lemma fbox_eta[simp]: "fbox (\<lambda>s. {s}) P = P"
-  unfolding fbox_def by simp
+definition fbox :: "('a \<Rightarrow> 'b set) \<Rightarrow> 'b pred \<Rightarrow> 'a pred" ("|_] _" [61,81] 82)
+  where "|F] P = (\<lambda>s. (\<forall>s'. s' \<in> F s \<longrightarrow> P s'))"
 
-lemma fbox_iso: "P \<le> Q \<Longrightarrow> fbox F P \<le> fbox F Q"
-  unfolding fbox_def by auto
-
-lemma fbox_def_univD: "fbox F P s = True \<Longrightarrow> (\<forall>s'. s' \<in> (F s) \<longrightarrow> P s')"
+lemma fbox_iso: "P \<le> Q \<Longrightarrow> |F] P \<le> |F] Q"
   unfolding fbox_def by auto
 
 lemma fbox_invariants: 
-  assumes "I \<le> fbox F I" and "J \<le> fbox F J"
-  shows "(\<lambda>s. I s \<and> J s) \<le> fbox F (\<lambda>s. I s \<and> J s)"
-    and "(\<lambda>s. I s \<or> J s) \<le> fbox F (\<lambda>s. I s \<or> J s)"
+  assumes "I \<le> |F] I" and "J \<le> |F] J"
+  shows "(\<lambda>s. I s \<and> J s) \<le> |F] (\<lambda>s. I s \<and> J s)"
+    and "(\<lambda>s. I s \<or> J s) \<le> |F] (\<lambda>s. I s \<or> J s)"
   using assms unfolding fbox_def by auto
+
+text \<open>Now, we compute wlps for specific programs.\<close>
+
+lemma fbox_eta[simp]: "fbox skip P = P"
+  unfolding fbox_def by simp
 
 text \<open>Next, we introduce assignments and their wlps.\<close>
 
@@ -42,7 +44,7 @@ definition vec_upd :: "('a^'n) \<Rightarrow> 'n \<Rightarrow> 'a \<Rightarrow> '
 definition assign :: "'n \<Rightarrow> ('a^'n \<Rightarrow> 'a) \<Rightarrow> ('a^'n) \<Rightarrow> ('a^'n) set" ("(2_ ::= _)" [70, 65] 61) 
   where "(x ::= e) = (\<lambda>s. {vec_upd s x (e s)})" 
 
-lemma fbox_assign[simp]: "fbox (x ::= e) Q = (\<lambda>s. Q (\<chi> j. ((($) s)(x := (e s))) j))"
+lemma fbox_assign[simp]: "|x ::= e] Q = (\<lambda>s. Q (\<chi> j. ((($) s)(x := (e s))) j))"
   unfolding vec_upd_def assign_def by (subst fbox_def) simp
 
 text \<open>The wlp of a (kleisli) composition is just the composition of the wlps.\<close>
@@ -53,12 +55,12 @@ definition kcomp :: "('a \<Rightarrow> 'b set) \<Rightarrow> ('b \<Rightarrow> '
 lemma kcomp_eq: "(f ; g) x = \<Union> {g y |y. y \<in> f x}"
   unfolding kcomp_def image_def by auto
 
-lemma fbox_kcomp: "fbox (G ; F) P = fbox G (fbox F P)"
+lemma fbox_kcomp[simp]: "|G ; F] P = |G] |F] P"
   unfolding fbox_def kcomp_def by auto
 
 lemma fbox_kcomp_ge:
-  assumes "P \<le> fbox F R" "R \<le> fbox G Q"
-  shows "P \<le> fbox (F ; G) Q"
+  assumes "P \<le> |G] R" "R \<le> |F] Q"
+  shows "P \<le> |G ; F] Q"
   apply(subst fbox_kcomp) 
   by (rule order.trans[OF assms(1)]) (rule fbox_iso[OF assms(2)])
 
@@ -68,32 +70,29 @@ definition ifthenelse :: "'a pred \<Rightarrow> ('a \<Rightarrow> 'b set) \<Righ
   ("IF _ THEN _ ELSE _" [64,64,64] 63) where 
   "IF P THEN X ELSE Y \<equiv> (\<lambda>s. if P s then X s else Y s)"
 
-lemma fbox_if_then_else:
-  "fbox (IF T THEN X ELSE Y) Q = (\<lambda>s. (T s \<longrightarrow> fbox X Q s) \<and> (\<not> T s \<longrightarrow> fbox Y Q s))"
+lemma fbox_if_then_else[simp]:
+  "|IF T THEN X ELSE Y] Q = (\<lambda>s. (T s \<longrightarrow> ( |X] Q) s) \<and> (\<not> T s \<longrightarrow> ( |Y] Q) s))"
   unfolding fbox_def ifthenelse_def by auto
 
 lemma fbox_if_then_else_ge:
-  assumes "(\<lambda>s. P s \<and> T s) \<le> fbox X Q"
-    and "(\<lambda>s. P s \<and> \<not> T s) \<le> fbox Y Q"
-  shows "P \<le> fbox (IF T THEN X ELSE Y) Q"
+  assumes "(\<lambda>s. P s \<and> T s) \<le> |X] Q"
+    and "(\<lambda>s. P s \<and> \<not> T s) \<le> |Y] Q"
+  shows "P \<le> |IF T THEN X ELSE Y] Q"
   using assms unfolding fbox_def ifthenelse_def by auto
 
 lemma fbox_if_then_elseI:
-  assumes "T s \<longrightarrow> fbox X Q s"
-    and "\<not> T s \<longrightarrow> fbox Y Q s"
-  shows "fbox (IF T THEN X ELSE Y) Q s"
+  assumes "T s \<longrightarrow> ( |X] Q) s"
+    and "\<not> T s \<longrightarrow> ( |Y] Q) s"
+  shows "( |IF T THEN X ELSE Y] Q) s"
   using assms unfolding fbox_def ifthenelse_def by auto
 
 text \<open>The final wlp we add is that of the finite iteration.\<close>
-
-abbreviation "skip \<equiv> (\<lambda>s. {s})"
 
 definition kpower :: "('a \<Rightarrow> 'a set) \<Rightarrow> nat \<Rightarrow> ('a \<Rightarrow> 'a set)" 
   where "kpower f n = (\<lambda>s. ((;) f ^^ n) skip s)"
 
 lemma kpower_base:
-  shows "kpower f 0 s = {s}"
-    and "kpower f (Suc 0) s = f s"
+  shows "kpower f 0 s = {s}" and "kpower f (Suc 0) s = f s"
   unfolding kpower_def by(auto simp: kcomp_eq)
 
 lemma kpower_simp: "kpower f (Suc n) s = (f ; kpower f n) s"
@@ -114,44 +113,54 @@ lemma kpower_inv:
   apply(subgoal_tac "I y", simp)
   using assms by blast
 
-lemma kstar_inv: "I \<le> fbox F I \<Longrightarrow> I \<le> fbox (F\<^sup>*) I"
+lemma kstar_inv: "I \<le> |F] I \<Longrightarrow> I \<le> |F\<^sup>*] I"
   unfolding kleene_star_def fbox_def apply clarsimp
   apply(unfold le_fun_def, subgoal_tac "\<forall>x. I x \<longrightarrow> (\<forall>s'. s' \<in> F x \<longrightarrow> I s')")
   apply(thin_tac "\<forall>x. I x \<le> (\<forall>s'. s' \<in> F x \<longrightarrow> I s')")
   using kpower_inv[of I F] by blast simp
 
 lemma fbox_kstarI:
-  assumes "P \<le> I" and "I \<le> Q" and "I \<le> fbox F I" 
-  shows "P \<le> fbox (F\<^sup>*) Q"
+  assumes "P \<le> I" and "I \<le> Q" and "I \<le> |F] I" 
+  shows "P \<le> |F\<^sup>*] Q"
 proof-
-  have "I \<le> fbox (F\<^sup>*) I"
+  have "I \<le> |F\<^sup>*] I"
     using assms(3) kstar_inv by blast
-  hence "P \<le> fbox (F\<^sup>*) I"
+  hence "P \<le> |F\<^sup>*] I"
     using assms(1) by auto
-  also have "fbox (F\<^sup>*) I \<le> fbox (F\<^sup>*) Q"
+  also have "|F\<^sup>*] I \<le> |F\<^sup>*] Q"
     by (rule fbox_iso[OF assms(2)])
   finally show ?thesis .
 qed
 
+definition loopi :: "('a \<Rightarrow> 'a set) \<Rightarrow> 'a pred \<Rightarrow> ('a \<Rightarrow> 'a set)" ("LOOP _ INV _ " [64,64] 63)
+  where "LOOP F INV I \<equiv> (F\<^sup>*)"
+
+lemma fbox_loopI: "P \<le> I \<Longrightarrow> I \<le> Q \<Longrightarrow> I \<le> |F] I \<Longrightarrow> P \<le> |LOOP F INV I] Q"
+  unfolding loopi_def using fbox_kstarI[of "P"] by simp
+
 
 section \<open>Verification of hybrid programs\<close>
 
-notation g_orbital ("(1x\<acute>=_ & _ on _ _ @ _)")
 
-abbreviation g_evol ::"(('a::banach)\<Rightarrow>'a) \<Rightarrow> 'a pred \<Rightarrow> 'a \<Rightarrow> 'a set" 
-  ("(1x\<acute>=_ & _)") where "(x\<acute>=f & G) s \<equiv> (x\<acute>=f & G on UNIV UNIV @ 0) s"
+subsection \<open>Verification by providing evolution\<close>
+
+definition g_evol :: "(real \<Rightarrow> 'a \<Rightarrow> 'a) \<Rightarrow> 'a pred \<Rightarrow> real set \<Rightarrow> ('a \<Rightarrow> 'a set)" ("EVOL")
+  where "EVOL \<phi> G T = (\<lambda>s. g_orbit (\<lambda>t. \<phi> t s) G T)"
+
+lemma fbox_g_evol[simp]: "|EVOL \<phi> G T] Q = (\<lambda>s. (\<forall>t\<in>T. (\<forall>\<tau>\<in>down T t. G (\<phi> \<tau> s)) \<longrightarrow> Q (\<phi> t s)))"
+  unfolding g_evol_def g_orbit_eq fbox_def by auto
 
 
 subsection \<open>Verification by providing solutions\<close>
 
-lemma fbox_g_orbital: "fbox (x\<acute>=f & G on T S @ t\<^sub>0) Q = 
-  (\<lambda>s. \<forall>X\<in>ivp_sols (\<lambda>t. f) T S t\<^sub>0 s. \<forall>t\<in>T. (\<forall>\<tau>\<in>down T t. G (X \<tau>)) \<longrightarrow> Q (X t))"
+lemma fbox_g_orbital: "|x\<acute>=f & G on T S @ t\<^sub>0] Q = 
+  (\<lambda>s. \<forall>X\<in>Sols (\<lambda>t. f) T S t\<^sub>0 s. \<forall>t\<in>T. (\<forall>\<tau>\<in>down T t. G (X \<tau>)) \<longrightarrow> Q (X t))"
   unfolding fbox_def g_orbital_eq by (auto simp: fun_eq_iff)
 
 context local_flow
 begin
 
-lemma fbox_g_orbit: "fbox (x\<acute>=f & G on T S @ 0) Q = 
+lemma fbox_g_ode: "|x\<acute>=f & G on T S @ 0] Q = 
   (\<lambda>s. s \<in> S \<longrightarrow> (\<forall>t\<in>T. (\<forall>\<tau>\<in>down T t. G (\<phi> \<tau> s)) \<longrightarrow> Q (\<phi> t s)))" (is "_ = ?wlp")
   unfolding fbox_g_orbital apply(rule ext, safe, clarsimp)
     apply(erule_tac x="\<lambda>t. \<phi> t s" in ballE)
@@ -160,7 +169,7 @@ lemma fbox_g_orbit: "fbox (x\<acute>=f & G on T S @ 0) Q =
   apply(subst eq_solution, simp_all add: ivp_sols_def)
   using init_time by auto
 
-lemma fbox_g_orbit_ivl: "t \<ge> 0 \<Longrightarrow> t \<in> T \<Longrightarrow> fbox (x\<acute>=f & G on {0..t} S @ 0) Q = 
+lemma fbox_g_ode_ivl: "t \<ge> 0 \<Longrightarrow> t \<in> T \<Longrightarrow> |x\<acute>=f & G on {0..t} S @ 0] Q = 
   (\<lambda>s. s \<in> S \<longrightarrow> (\<forall>t\<in>{0..t}. (\<forall>\<tau>\<in>{0..t}. G (\<phi> \<tau> s)) \<longrightarrow> Q (\<phi> t s)))"
   unfolding fbox_g_orbital apply(rule ext, clarsimp, safe)
     apply(erule_tac x="\<lambda>t. \<phi> t s" in ballE, force)
@@ -173,29 +182,45 @@ lemma fbox_g_orbit_ivl: "t \<ge> 0 \<Longrightarrow> t \<in> T \<Longrightarrow>
   using interval_time init_time apply (meson is_interval_1 order_trans) 
   using init_time by force
 
-lemma fbox_orbit: "fbox \<gamma>\<^sup>\<phi> Q = (\<lambda>s. s \<in> S \<longrightarrow> (\<forall> t \<in> T. Q (\<phi> t s)))"
-  unfolding orbit_def fbox_g_orbit by simp
+lemma fbox_orbit: "|\<gamma>\<^sup>\<phi>] Q = (\<lambda>s. s \<in> S \<longrightarrow> (\<forall> t \<in> T. Q (\<phi> t s)))"
+  unfolding orbit_def fbox_g_ode by simp
 
 end
 
 
 subsection\<open> Verification with differential invariants \<close>
 
+definition g_ode_inv :: "(('a::banach)\<Rightarrow>'a) \<Rightarrow> 'a pred \<Rightarrow> real set \<Rightarrow> 'a set \<Rightarrow> 
+  real \<Rightarrow> 'a pred \<Rightarrow> ('a \<Rightarrow> 'a set)" ("(1x\<acute>=_ & _ on _ _ @ _ DINV _ )") 
+  where "(x\<acute>= f & G on T S @ t\<^sub>0 DINV I) = (x\<acute>= f & G on T S @ t\<^sub>0)"
+
 lemma fbox_g_orbital_guard: 
   assumes "H = (\<lambda>s. G s \<and> Q s)"
-  shows "fbox (x\<acute>=f & G on T S @ t\<^sub>0) H = fbox (x\<acute>=f & G on T S @ t\<^sub>0) Q"
+  shows "|x\<acute>=f & G on T S @ t\<^sub>0] Q = |x\<acute>=f & G on T S @ t\<^sub>0] H "
   unfolding fbox_g_orbital using assms by auto
 
 lemma fbox_g_orbital_inv:
-  assumes "P \<le> I" and "I \<le> fbox (x\<acute>=f & G on T S @ t\<^sub>0) I" and "I \<le> Q"
-  shows "P \<le> fbox (x\<acute>=f & G on T S @ t\<^sub>0) Q"
+  assumes "P \<le> I" and "I \<le> |x\<acute>=f & G on T S @ t\<^sub>0] I" and "I \<le> Q"
+  shows "P \<le> |x\<acute>=f & G on T S @ t\<^sub>0] Q"
   using assms(1) apply(rule order.trans)
   using assms(2) apply(rule order.trans)
   by (rule fbox_iso[OF assms(3)])
 
-lemma fbox_diff_inv: 
-  "(I \<le> fbox (x\<acute>=f & G on T S @ t\<^sub>0) I) = diff_invariant I f T S t\<^sub>0 G"
+lemma fbox_diff_inv[simp]: 
+  "(I \<le> |x\<acute>=f & G on T S @ t\<^sub>0] I) = diff_invariant I f T S t\<^sub>0 G"
   by (auto simp: diff_invariant_def ivp_sols_def fbox_def g_orbital_eq)
 
+lemma fbox_g_odei: "P \<le> I \<Longrightarrow> I \<le> |x\<acute>= f & G on T S @ t\<^sub>0] I \<Longrightarrow> (\<lambda>s. I s \<and> G s) \<le> Q \<Longrightarrow> 
+  P \<le> |x\<acute>= f & G on T S @ t\<^sub>0 DINV I] Q"
+  unfolding g_ode_inv_def apply(rule_tac b="|x\<acute>= f & G on T S @ t\<^sub>0] I" in order.trans)
+   apply(rule_tac I="I" in fbox_g_orbital_inv, simp_all)
+  apply(subst fbox_g_orbital_guard, simp)
+  by (rule fbox_iso, force)
+
+abbreviation g_global_orbit ::"(('a::banach)\<Rightarrow>'a) \<Rightarrow> 'a pred \<Rightarrow> 'a \<Rightarrow> 'a set" 
+  ("(1x\<acute>=_ & _)") where "(x\<acute>=f & G) \<equiv> (x\<acute>=f & G on UNIV UNIV @ 0)"
+
+abbreviation g_global_ode_inv ::"(('a::banach)\<Rightarrow>'a) \<Rightarrow> 'a pred \<Rightarrow> 'a pred \<Rightarrow> 'a \<Rightarrow> 'a set" 
+  ("(1x\<acute>=_ & _ DINV _)") where "(x\<acute>=f & G DINV I) \<equiv> (x\<acute>=f & G on UNIV UNIV @ 0 DINV I)"
 
 end
