HybridVerifVecs/nd_funs/cat2ndfun.thy
@@ -20,7 +20,6 @@ type_synonym 'a pred = "'a \<Rightarrow> bool"
 notation Abs_nd_fun ("_\<^sup>\<bullet>" [101] 100) 
      and Rep_nd_fun ("_\<^sub>\<bullet>" [101] 100)
      and fbox ("wp")
-     and qstar ("loop")
 
 section\<open> Nondeterministic Functions \<close>
 
@@ -122,6 +121,14 @@ lemma ads_d_p2ndf_simps[simp]:
    apply(simp_all add: antidomain_op_nd_fun_def)
   by (rule nd_fun_ext, force)+
 
+lemma p2ndf_times[simp]: "\<lceil>P\<rceil> \<cdot> \<lceil>Q\<rceil> = \<lceil>\<lambda>s. P s \<and> Q s\<rceil>"
+  apply(clarsimp simp: times_nd_fun_def nd_fun_eq_iff[symmetric] kcomp_def)
+  by (rule antisym, simp_all add: image_def subset_eq)
+
+lemma p2ndf_plus[simp]: "\<lceil>P\<rceil> + \<lceil>Q\<rceil> = \<lceil>\<lambda>s. P s \<or> Q s\<rceil>"
+  apply(clarsimp simp: plus_nd_fun_def nd_fun_eq_iff[symmetric])
+  by (rule antisym, auto simp: image_def subset_eq)
+
 lemma ad_p2ndf[simp]: "ad \<lceil>P\<rceil> = \<lceil>\<lambda>s. \<not> P s\<rceil>"
   unfolding antidomain_op_nd_fun_def by(rule nd_fun_ext, auto)
 
@@ -203,6 +210,9 @@ text\<open> The @{text "wp"} of the composition was already obtained in KAD.Anti
 abbreviation seq_comp :: "'a nd_fun \<Rightarrow> 'a nd_fun \<Rightarrow> 'a nd_fun" (infixl ";" 75)
   where "f ; g \<equiv> f \<cdot> g"
 
+lemma wlp_seq_comp[simp]: "wp (F ; G) Q = wp F (wp G Q)"
+  by (simp add: fbox_mult)
+
 text\<open> We also have an implementation of the conditional operator and its @{text "wp"}. \<close>
 
 definition (in antidomain_kleene_algebra) cond :: "'a \<Rightarrow> 'a \<Rightarrow> 'a \<Rightarrow> 'a" 
@@ -229,10 +239,30 @@ lemma wp_if_then_elseI:
 
 text\<open> We also deal with finite iteration. \<close>
 
-lemma (in antidomain_kleene_algebra) fbox_starI: 
+context antidomain_kleene_algebra
+begin
+
+lemma plus_inv: "i \<le> |x] i \<Longrightarrow> j \<le> |x] j \<Longrightarrow> (i + j) \<le> |x] (i + j)"
+  by (metis ads_d_def dka.dsr5 fbox_simp fbox_subdist join.sup_mono order_trans)
+
+lemma fbox_frame: "d p \<cdot> x \<le> x \<cdot> d p \<Longrightarrow> d q \<le> |x] t \<Longrightarrow> d p \<cdot> d q \<le> |x] (d p \<cdot> d t)"    
+  using dual.mult_isol_var fbox_add1 fbox_demodalisation3 fbox_simp by auto
+
+lemma mult_inv: "d i \<le> |x] d i \<Longrightarrow> d j \<le> |x] d j \<Longrightarrow> (d i \<cdot> d j) \<le> |x] (d i \<cdot> d j)"
+  using local.fbox_demodalisation3 fbox_frame fbox_simp by auto
+
+lemma (in antidomain_kleene_algebra) fbox_stari: 
   assumes "d p \<le> d i" and "d i \<le> |x] i" and "d i \<le> d q"
   shows "d p \<le> |x\<^sup>\<star>] q"
-  by (meson assms local.dual_order.trans local.fbox_iso local.fbox_star_induct_var)
+  by (meson assms local.dual_order.trans fbox_iso fbox_star_induct_var)
+
+definition loopi :: "'a \<Rightarrow> 'a \<Rightarrow> 'a" ("loop _ inv _ " [64,64] 63)
+  where "loop x inv i = x\<^sup>\<star>"
+
+lemma fbox_loopi: "d p \<le> d i \<Longrightarrow> d i \<le> |x] i \<Longrightarrow> d i \<le> d q \<Longrightarrow> d p \<le> |loop x inv i] q"
+  unfolding loopi_def using fbox_stari by blast
+
+end
 
 lemma ads_d_mono: "x \<le> y \<Longrightarrow> d x \<le> d y"
   by (metis ads_d_def fbox_antitone_var fbox_dom)
@@ -245,7 +275,7 @@ lemma nd_fun_top_ads_d:"(x::'a nd_fun) \<le> 1 \<Longrightarrow> d x = x"
 
 lemma wp_starI:
   assumes "P \<le> I" and "I \<le> Q" and "I \<le> wp F I"
-  shows "P \<le> wp (loop (F::'a nd_fun)) Q"
+  shows "P \<le> wp (qstar (F::'a nd_fun)) Q"
 proof-
   have "P \<le> 1"
     using assms(1,3) by (metis a_subid basic_trans_rules(23) fbox_def) 
@@ -255,33 +285,46 @@ proof-
   hence "d P \<le> d I \<and> d I \<le> wp F I \<and> d I \<le> d Q"
     using assms by (metis (no_types) ads_d_mono assms)
   hence "d P \<le> wp (F\<^sup>\<star>) Q"
-    by(simp add: fbox_starI[of _ I])
-  thus "P \<le> wp (loop F) Q"
+    by(simp add: fbox_stari[of _ I])
+  thus "P \<le> wp (qstar F) Q"
     using \<open>d P = P\<close> by (transfer, simp)
 qed
+
+abbreviation loopi_sugar :: "'a nd_fun \<Rightarrow> 'a pred \<Rightarrow> 'a nd_fun" ("LOOP _ INV _ " [64,64] 63)
+  where "LOOP R INV I \<equiv> loopi R \<lceil>I\<rceil>"
+
+lemma wp_loopI: "\<lceil>P\<rceil> \<le> \<lceil>I\<rceil> \<Longrightarrow> \<lceil>I\<rceil> \<le> \<lceil>Q\<rceil> \<Longrightarrow> \<lceil>I\<rceil> \<le> wp R \<lceil>I\<rceil> \<Longrightarrow> \<lceil>P\<rceil> \<le> wp (LOOP R INV I) \<lceil>Q\<rceil>"
+  using fbox_loopi[of "\<lceil>P\<rceil>"] by auto
 
 
 section\<open> Verification of hybrid programs \<close>
 
-abbreviation g_evolution ::"(('a::banach)\<Rightarrow>'a) \<Rightarrow> 'a pred \<Rightarrow> real set \<Rightarrow> 'a set \<Rightarrow> 
-  real \<Rightarrow> 'a nd_fun" ("(1x\<acute>=_ & _ on _ _ @ _)") 
-  where "(x\<acute>=f & G on T S @ t\<^sub>0) \<equiv> (\<lambda> s. g_orbital f G T S t\<^sub>0 s)\<^sup>\<bullet>"
+
+subsection \<open>Verification by providing evolution\<close>
+
+definition g_evol :: "(real \<Rightarrow> 'a \<Rightarrow> 'a) \<Rightarrow> 'a pred \<Rightarrow> real set \<Rightarrow> 'a nd_fun" ("EVOL")
+  where "EVOL \<phi> G T = (\<lambda>s. g_orbit (\<lambda>t. \<phi> t s) G T)\<^sup>\<bullet>"
+
+lemma wp_g_dyn[simp]: "wp (EVOL \<phi> G T) \<lceil>Q\<rceil> = \<lceil>\<lambda>s. \<forall>t\<in>T. (\<forall>\<tau>\<in>down T t. G (\<phi> \<tau> s)) \<longrightarrow> Q (\<phi> t s)\<rceil>"
+  unfolding wp_nd_fun g_evol_def g_orbit_eq by (auto simp: fun_eq_iff)
 
 
 subsection \<open>Verification by providing solutions\<close>
 
-text\<open>The wlp of evolution commands. \<close>
+definition g_ode ::"(('a::banach)\<Rightarrow>'a) \<Rightarrow> 'a pred \<Rightarrow> real set \<Rightarrow> 'a set \<Rightarrow> 
+  real \<Rightarrow> 'a nd_fun" ("(1x\<acute>= _ & _ on _ _ @ _)") 
+  where "(x\<acute>= f & G on T S @ t\<^sub>0) \<equiv> (\<lambda> s. g_orbital f G T S t\<^sub>0 s)\<^sup>\<bullet>"
 
-lemma wp_g_evolution: "wp (x\<acute>=f & G on T S @ t\<^sub>0) \<lceil>Q\<rceil>= 
+lemma wp_g_orbital: "wp (x\<acute>= f & G on T S @ t\<^sub>0) \<lceil>Q\<rceil>= 
   \<lceil>\<lambda> s. \<forall>X\<in>ivp_sols (\<lambda>t. f) T S t\<^sub>0 s. \<forall>t\<in>T. (\<forall>\<tau>\<in>down T t. G (X \<tau>)) \<longrightarrow> Q (X t)\<rceil>"
-  unfolding g_orbital_eq(1) wp_nd_fun by (auto simp: fun_eq_iff image_le_pred)
+  unfolding g_orbital_eq(1) wp_nd_fun g_ode_def by (auto simp: fun_eq_iff image_le_pred)
 
 context local_flow
 begin
 
-lemma wp_g_orbit: "wp (x\<acute>=f & G on T S @ 0) \<lceil>Q\<rceil> = 
+lemma wp_g_ode: "wp (x\<acute>= f & G on T S @ 0) \<lceil>Q\<rceil> = 
   \<lceil>\<lambda> s. s \<in> S \<longrightarrow> (\<forall>t\<in>T. (\<forall>\<tau>\<in>down T t. G (\<phi> \<tau> s)) \<longrightarrow> Q (\<phi> t s))\<rceil>"
-  unfolding wp_g_evolution apply(clarsimp, simp add: fun_eq_iff, safe)
+  unfolding wp_g_orbital apply(clarsimp, simp add: fun_eq_iff, safe)
     apply(erule_tac x="\<lambda>t. \<phi> t x" in ballE)
   using in_ivp_sols apply(force, force, force simp: init_time ivp_sols_def)
   apply(subgoal_tac "\<forall>\<tau>\<in>down T t. X \<tau> = \<phi> \<tau> x", simp_all, clarsimp)
@@ -289,28 +332,39 @@ lemma wp_g_orbit: "wp (x\<acute>=f & G on T S @ 0) \<lceil>Q\<rceil> =
   using init_time by auto
 
 lemma wp_orbit: "wp (\<gamma>\<^sup>\<phi>\<^sup>\<bullet>) \<lceil>Q\<rceil> = \<lceil>\<lambda> s. s \<in> S \<longrightarrow> (\<forall> t \<in> T. Q (\<phi> t s))\<rceil>"
-  unfolding orbit_def wp_g_orbit by auto
+  unfolding orbit_def wp_g_ode g_ode_def[symmetric] by auto
 
 end
 
+
 subsection\<open> Verification with differential invariants \<close>
 
-lemma wp_g_evolution_guard: 
-  assumes "H = (\<lambda>s. G s \<and> Q s)"
-  shows "wp (x\<acute>=f & G on T S @ t\<^sub>0) \<lceil>H\<rceil> = wp (x\<acute>=f & G on T S @ t\<^sub>0) \<lceil>Q\<rceil>"
-  unfolding wp_g_evolution using assms by auto
+definition g_ode_inv :: "(('a::banach)\<Rightarrow>'a) \<Rightarrow> 'a pred \<Rightarrow> real set \<Rightarrow> 'a set \<Rightarrow> 
+  real \<Rightarrow> 'a pred \<Rightarrow> 'a nd_fun" ("(1x\<acute>=_ & _ on _ _ @ _ DINV _ )") 
+  where "(x\<acute>= f & G on T S @ t\<^sub>0 DINV I) = (x\<acute>= f & G on T S @ t\<^sub>0)"
 
-lemma wp_g_evolution_inv:
-  assumes "\<lceil>P\<rceil> \<le> \<lceil>I\<rceil>" and "\<lceil>I\<rceil> \<le> wp (x\<acute>=f & G on T S @ t\<^sub>0) \<lceil>I\<rceil>" and "\<lceil>I\<rceil> \<le> \<lceil>Q\<rceil>"
-  shows "\<lceil>P\<rceil> \<le> wp (x\<acute>=f & G on T S @ t\<^sub>0) \<lceil>Q\<rceil>"
+lemma wp_g_orbital_guard: 
+  assumes "H = (\<lambda>s. G s \<and> Q s)"
+  shows "wp (x\<acute>= f & G on T S @ t\<^sub>0) \<lceil>Q\<rceil> = wp (x\<acute>= f & G on T S @ t\<^sub>0) \<lceil>H\<rceil>"
+  unfolding wp_g_orbital using assms by auto
+
+lemma wp_g_orbital_inv:
+  assumes "\<lceil>P\<rceil> \<le> \<lceil>I\<rceil>" and "\<lceil>I\<rceil> \<le> wp (x\<acute>= f & G on T S @ t\<^sub>0) \<lceil>I\<rceil>" and "\<lceil>I\<rceil> \<le> \<lceil>Q\<rceil>"
+  shows "\<lceil>P\<rceil> \<le> wp (x\<acute>= f & G on T S @ t\<^sub>0) \<lceil>Q\<rceil>"
   using assms(1) apply(rule order.trans)
   using assms(2) apply(rule order.trans)
   apply(rule fbox_iso)
   using assms(3) by auto
 
-lemma wp_diff_inv: "(\<lceil>I\<rceil> \<le> wp (x\<acute>=f & G on T S @ t\<^sub>0) \<lceil>I\<rceil>) = diff_invariant I f T S t\<^sub>0 G"
-  unfolding diff_invariant_eq wp_g_evolution image_le_pred by(auto simp: fun_eq_iff)
+lemma wp_diff_inv[simp]: "(\<lceil>I\<rceil> \<le> wp (x\<acute>= f & G on T S @ t\<^sub>0) \<lceil>I\<rceil>) = diff_invariant I f T S t\<^sub>0 G"
+  unfolding diff_invariant_eq wp_g_orbital image_le_pred by(auto simp: fun_eq_iff)
 
+lemma wp_g_odei: "\<lceil>P\<rceil> \<le> \<lceil>I\<rceil> \<Longrightarrow> \<lceil>I\<rceil> \<le> wp (x\<acute>= f & G on T S @ t\<^sub>0) \<lceil>I\<rceil> \<Longrightarrow> \<lceil>\<lambda>s. I s \<and> G s\<rceil> \<le> \<lceil>Q\<rceil> \<Longrightarrow> 
+  \<lceil>P\<rceil> \<le> wp (x\<acute>= f & G on T S @ t\<^sub>0 DINV I) \<lceil>Q\<rceil>"
+  unfolding g_ode_inv_def apply(rule_tac b="wp (x\<acute>= f & G on T S @ t\<^sub>0) \<lceil>I\<rceil>" in order.trans)
+   apply(rule_tac I="I" in wp_g_orbital_inv, simp_all)
+  apply(subst wp_g_orbital_guard, simp)
+  by (rule fbox_iso, simp)
 
 subsection\<open> Derivation of the rules of dL \<close>
 
@@ -322,20 +376,21 @@ lemma diff_solve_axiom:
   assumes "0 \<in> T" and "is_interval T" "open T"
   shows "wp (x\<acute>=(\<lambda>s. c) & G on T UNIV @ 0) \<lceil>Q\<rceil> = 
   \<lceil>\<lambda> s. \<forall>t\<in>T. (\<P> (\<lambda> t. s + t *\<^sub>R c) (down T t) \<subseteq> {s. G s}) \<longrightarrow> Q (s + t *\<^sub>R c)\<rceil>"
-  apply(subst local_flow.wp_g_orbit[where f="\<lambda>s. c" and \<phi>="(\<lambda> t s. s + t *\<^sub>R c)"])
+  apply(subst local_flow.wp_g_ode[where f="\<lambda>s. c" and \<phi>="(\<lambda> t s. s + t *\<^sub>R c)"])
   using line_is_local_flow[OF assms] unfolding image_le_pred by auto
 
 lemma diff_solve_rule:
   assumes "local_flow f T UNIV \<phi>"
     and "\<forall>s. P s \<longrightarrow> (\<forall> t\<in>T. (\<P> (\<lambda>t. \<phi> t s) (down T t) \<subseteq> {s. G s}) \<longrightarrow> Q (\<phi> t s))"
-  shows "\<lceil>P\<rceil> \<le> wp (x\<acute>=f & G on T UNIV @ 0) \<lceil>Q\<rceil>"
-  using assms by(subst local_flow.wp_g_orbit, auto)
+  shows "\<lceil>P\<rceil> \<le> wp (x\<acute>= f & G on T UNIV @ 0) \<lceil>Q\<rceil>"
+  using assms by(subst local_flow.wp_g_ode, auto)
 
-lemma diff_weak_axiom: "wp (x\<acute>=f & G on T S @ t\<^sub>0) \<lceil>Q\<rceil> = wp (x\<acute>=f & G on T S @ t\<^sub>0) \<lceil>\<lambda> s. G s \<longrightarrow> Q s\<rceil>"
-  unfolding wp_g_evolution image_def by force
+lemma diff_weak_axiom: 
+  "wp (x\<acute>= f & G on T S @ t\<^sub>0) \<lceil>Q\<rceil> = wp (x\<acute>= f & G on T S @ t\<^sub>0) \<lceil>\<lambda> s. G s \<longrightarrow> Q s\<rceil>"
+  unfolding wp_g_orbital image_def by force
 
-lemma diff_weak_rule: "\<lceil>G\<rceil> \<le> \<lceil>Q\<rceil> \<Longrightarrow> \<lceil>P\<rceil> \<le> wp (x\<acute>=f & G on T S @ t\<^sub>0) \<lceil>Q\<rceil>"
-  by (subst wp_nd_fun) (auto simp: g_orbital_eq)
+lemma diff_weak_rule: "\<lceil>G\<rceil> \<le> \<lceil>Q\<rceil> \<Longrightarrow> \<lceil>P\<rceil> \<le> wp (x\<acute>= f & G on T S @ t\<^sub>0) \<lceil>Q\<rceil>"
+  by (subst wp_g_orbital) (auto simp: g_ode_def)
 
 lemma wp_nd_fun_etaD: "wp (F\<^sup>\<bullet>) \<lceil>P\<rceil> = \<eta>\<^sup>\<bullet> \<Longrightarrow>  (\<forall>y. y \<in> (F x) \<longrightarrow> P y)"
 proof
@@ -349,7 +404,7 @@ proof
 qed
 
 lemma wp_g_orbit_IdD:
-  assumes "wp (x\<acute>=f & G on T S @ t\<^sub>0) \<lceil>C\<rceil> = \<eta>\<^sup>\<bullet>"
+  assumes "wp (x\<acute>= f & G on T S @ t\<^sub>0) \<lceil>C\<rceil> = \<eta>\<^sup>\<bullet>"
     and "\<forall>\<tau>\<in>(down T t). x \<tau> \<in> g_orbital f G T S t\<^sub>0 s"
   shows "\<forall>\<tau>\<in>(down T t). C (x \<tau>)"
 proof
@@ -357,18 +412,20 @@ proof
   hence "x \<tau> \<in> g_orbital f G T S t\<^sub>0 s" 
     using assms(2) by blast
   also have "\<forall>y. y \<in> (g_orbital f G T S t\<^sub>0 s) \<longrightarrow> C y" 
-    using assms(1) unfolding wp_nd_fun by (subst (asm) nd_fun_eq_iff[symmetric]) auto
+    using assms(1) unfolding wp_nd_fun g_ode_def 
+    by (subst (asm) nd_fun_eq_iff[symmetric]) auto
   ultimately show "C (x \<tau>)" 
     by blast
 qed
 
 lemma diff_cut_axiom:
   assumes Thyp: "is_interval T" "t\<^sub>0 \<in> T"
-    and "wp (x\<acute>=f & G on T S @ t\<^sub>0) \<lceil>C\<rceil> = \<eta>\<^sup>\<bullet>"
-  shows "wp (x\<acute>=f & G on T S @ t\<^sub>0) \<lceil>Q\<rceil> = wp (x\<acute>=f & (\<lambda>s. G s \<and> C s) on T S @ t\<^sub>0) \<lceil>Q\<rceil>"
-proof(rule_tac f="\<lambda> x. wp x \<lceil>Q\<rceil>" in HOL.arg_cong, rule nd_fun_ext, rule subset_antisym, simp_all)
-  fix s 
-  {fix s' assume "s' \<in> g_orbital f G T S t\<^sub>0 s"
+    and "wp (x\<acute>= f & G on T S @ t\<^sub>0) \<lceil>C\<rceil> = \<eta>\<^sup>\<bullet>"
+  shows "wp (x\<acute>= f & G on T S @ t\<^sub>0) \<lceil>Q\<rceil> = wp (x\<acute>= f & (\<lambda>s. G s \<and> C s) on T S @ t\<^sub>0) \<lceil>Q\<rceil>"
+proof(rule_tac f="\<lambda> x. wp x \<lceil>Q\<rceil>" in HOL.arg_cong, rule nd_fun_ext, rule subset_antisym)
+  fix s show "((x\<acute>= f & G on T S @ t\<^sub>0)\<^sub>\<bullet>) s \<subseteq> ((x\<acute>= f & (\<lambda>s. G s \<and> C s) on T S @ t\<^sub>0)\<^sub>\<bullet>) s"
+  proof(clarsimp simp: g_ode_def)
+    fix s' assume "s' \<in> g_orbital f G T S t\<^sub>0 s"
     then obtain \<tau>::real and X where x_ivp: "X \<in> ivp_sols (\<lambda>t. f) T S t\<^sub>0 s" 
       and "X \<tau> = s'" and "\<tau> \<in> T" and guard_x:"(\<P> X (down T \<tau>) \<subseteq> {s. G s})"
       using g_orbitalD[of s' "f" G T S t\<^sub>0 s] by blast
@@ -380,40 +437,41 @@ proof(rule_tac f="\<lambda> x. wp x \<lceil>Q\<rceil>" in HOL.arg_cong, rule nd_
       using g_orbitalI[OF x_ivp] by (metis (mono_tags, lifting))
     hence "\<forall>t\<in>(down T \<tau>). C (X t)" 
       using wp_g_orbit_IdD[OF assms(3)] by blast
-    hence "s' \<in> g_orbital f (\<lambda>s. G s \<and> C s) T S t\<^sub>0 s"
+    thus "s' \<in> g_orbital f (\<lambda>s. G s \<and> C s) T S t\<^sub>0 s"
       using g_orbitalI[OF x_ivp \<open>\<tau> \<in> T\<close>] guard_x \<open>X \<tau> = s'\<close> 
-      unfolding image_le_pred by fastforce}
-  thus "g_orbital f G T S t\<^sub>0 s \<subseteq> g_orbital f (\<lambda>s. G s \<and> C s) T S t\<^sub>0 s"
-    by blast
+      unfolding image_le_pred by fastforce
+  qed
 next 
-  fix s
-  show "g_orbital f (\<lambda>s. G s \<and> C s) T S t\<^sub>0 s \<subseteq> g_orbital f G T S t\<^sub>0 s" 
-    by (auto simp: g_orbital_eq)
+  fix s show "((x\<acute>= f & \<lambda>s. G s \<and> C s on T S @ t\<^sub>0)\<^sub>\<bullet>) s \<subseteq> ((x\<acute>= f & G on T S @ t\<^sub>0)\<^sub>\<bullet>) s" 
+    by (auto simp: g_orbital_eq g_ode_def)
 qed
 
 lemma diff_cut_rule:
   assumes Thyp: "is_interval T" "t\<^sub>0 \<in> T"
-    and wp_C: "\<lceil>P\<rceil> \<le> wp (x\<acute>=f & G on T S @ t\<^sub>0) \<lceil>C\<rceil>"
-    and wp_Q: "\<lceil>P\<rceil> \<le> wp (x\<acute>=f & (\<lambda>s. G s \<and> C s) on T S @ t\<^sub>0) \<lceil>Q\<rceil>"
-  shows "\<lceil>P\<rceil> \<le> wp (x\<acute>=f & G on T S @ t\<^sub>0) \<lceil>Q\<rceil>"
-proof(simp add: wp_nd_fun g_orbital_eq image_le_pred, clarsimp)
+    and wp_C: "\<lceil>P\<rceil> \<le> wp (x\<acute>= f & G on T S @ t\<^sub>0) \<lceil>C\<rceil>"
+    and wp_Q: "\<lceil>P\<rceil> \<le> wp (x\<acute>= f & (\<lambda>s. G s \<and> C s) on T S @ t\<^sub>0) \<lceil>Q\<rceil>"
+  shows "\<lceil>P\<rceil> \<le> wp (x\<acute>= f & G on T S @ t\<^sub>0) \<lceil>Q\<rceil>"
+proof(simp add: wp_nd_fun g_orbital_eq image_le_pred g_ode_def, clarsimp)
   fix t::real and X::"real \<Rightarrow> 'a" and s assume "P s" and "t \<in> T"
     and x_ivp:"X \<in> ivp_sols (\<lambda>t. f) T S t\<^sub>0 s" 
     and guard_x:"\<forall>x. x \<in> T \<and> x \<le> t \<longrightarrow> G (X x)"
   have "\<forall>t\<in>(down T t). X t \<in> g_orbital f G T S t\<^sub>0 s"
     using g_orbitalI[OF x_ivp] guard_x unfolding image_le_pred by auto
   hence "\<forall>t\<in>(down T t). C (X t)" 
-    using wp_C \<open>P s\<close> by (subst (asm) wp_nd_fun, auto)
+    using wp_C \<open>P s\<close> by (subst (asm) wp_nd_fun2, auto simp: g_ode_def)
   hence "X t \<in> g_orbital f (\<lambda>s. G s \<and> C s) T S t\<^sub>0 s"
     using guard_x \<open>t \<in> T\<close> by (auto intro!: g_orbitalI x_ivp)
   thus "Q (X t)"
-    using \<open>P s\<close> wp_Q by (subst (asm) wp_nd_fun) auto
+    using \<open>P s\<close> wp_Q by (subst (asm) wp_nd_fun2) (auto simp: g_ode_def)
 qed
 
 text\<open>The rules of dL\<close>
 
-abbreviation g_evol ::"(('a::banach)\<Rightarrow>'a) \<Rightarrow> 'a pred \<Rightarrow> 'a nd_fun" ("(1x\<acute>=_ & _)") 
-  where "(x\<acute>=f & G) \<equiv> (x\<acute>=f & G on UNIV UNIV @ 0)"
+abbreviation g_global_ode ::"(('a::banach)\<Rightarrow>'a) \<Rightarrow> 'a pred \<Rightarrow> 'a nd_fun" ("(1x\<acute>=_ & _)") 
+  where "(x\<acute>= f & G) \<equiv> (x\<acute>= f & G on UNIV UNIV @ 0)"
+
+abbreviation g_global_ode_inv :: "(('a::banach)\<Rightarrow>'a) \<Rightarrow> 'a pred \<Rightarrow> 'a pred \<Rightarrow> 'a nd_fun" 
+  ("(1x\<acute>=_ & _ DINV _)") where "(x\<acute>= f & G DINV I) \<equiv> (x\<acute>= f & G on UNIV UNIV @ 0 DINV I)"
 
 lemma DS: 
   fixes c::"'a::{heine_borel, banach}"
@@ -423,33 +481,33 @@ lemma DS:
 lemma solve:
   assumes "local_flow f UNIV UNIV \<phi>"
     and "\<forall>s. P s \<longrightarrow> (\<forall>t. (\<forall>\<tau>\<le>t. G (\<phi> \<tau> s)) \<longrightarrow> Q (\<phi> t s))"
-  shows "\<lceil>P\<rceil> \<le> wp (x\<acute>=f & G) \<lceil>Q\<rceil>"
+  shows "\<lceil>P\<rceil> \<le> wp (x\<acute>= f & G) \<lceil>Q\<rceil>"
   apply(rule diff_solve_rule[OF assms(1)])
   using assms(2) unfolding image_le_pred by simp
 
-lemma DW: "wp (x\<acute>=f & G) \<lceil>Q\<rceil> = wp (x\<acute>=f & G) \<lceil>\<lambda>s. G s \<longrightarrow> Q s\<rceil>"
+lemma DW: "wp (x\<acute>= f & G) \<lceil>Q\<rceil> = wp (x\<acute>= f & G) \<lceil>\<lambda>s. G s \<longrightarrow> Q s\<rceil>"
   by (rule diff_weak_axiom)
   
-lemma dW: "\<lceil>G\<rceil> \<le> \<lceil>Q\<rceil> \<Longrightarrow> \<lceil>P\<rceil> \<le> wp (x\<acute>=f & G) \<lceil>Q\<rceil>"
+lemma dW: "\<lceil>G\<rceil> \<le> \<lceil>Q\<rceil> \<Longrightarrow> \<lceil>P\<rceil> \<le> wp (x\<acute>= f & G) \<lceil>Q\<rceil>"
   by (rule diff_weak_rule)
 
 lemma DC:
-  assumes "wp (x\<acute>=f & G) \<lceil>C\<rceil> = \<eta>\<^sup>\<bullet>"
-  shows "wp (x\<acute>=f & G) \<lceil>Q\<rceil> = wp (x\<acute>=f & (\<lambda>s. G s \<and> C s)) \<lceil>Q\<rceil>"
+  assumes "wp (x\<acute>= f & G) \<lceil>C\<rceil> = \<eta>\<^sup>\<bullet>"
+  shows "wp (x\<acute>= f & G) \<lceil>Q\<rceil> = wp (x\<acute>= f & (\<lambda>s. G s \<and> C s)) \<lceil>Q\<rceil>"
   apply (rule diff_cut_axiom) 
   using assms by auto
 
 lemma dC:
-  assumes "\<lceil>P\<rceil> \<le> wp (x\<acute>=f & G) \<lceil>C\<rceil>"
-    and "\<lceil>P\<rceil> \<le> wp (x\<acute>=f & (\<lambda>s. G s \<and> C s)) \<lceil>Q\<rceil>"
-  shows "\<lceil>P\<rceil> \<le> wp (x\<acute>=f & G) \<lceil>Q\<rceil>"
+  assumes "\<lceil>P\<rceil> \<le> wp (x\<acute>= f & G) \<lceil>C\<rceil>"
+    and "\<lceil>P\<rceil> \<le> wp (x\<acute>= f & (\<lambda>s. G s \<and> C s)) \<lceil>Q\<rceil>"
+  shows "\<lceil>P\<rceil> \<le> wp (x\<acute>= f & G) \<lceil>Q\<rceil>"
   apply(rule diff_cut_rule)
   using assms by auto
 
 lemma dI:
   assumes "\<lceil>P\<rceil> \<le> \<lceil>I\<rceil>" and "diff_invariant I f UNIV UNIV 0 G" and "\<lceil>I\<rceil> \<le> \<lceil>Q\<rceil>"
-  shows "\<lceil>P\<rceil> \<le> wp (x\<acute>=f & G) \<lceil>Q\<rceil>"
-  apply(rule wp_g_evolution_inv[OF assms(1) _ assms(3)])
+  shows "\<lceil>P\<rceil> \<le> wp (x\<acute>= f & G) \<lceil>Q\<rceil>"
+  apply(rule wp_g_orbital_inv[OF assms(1) _ assms(3)])
   unfolding wp_diff_inv using assms(2) .
 
 end
