HybridVerifVecs/rels/cat2rel.thy
@@ -19,7 +19,6 @@ no_notation Archimedean_Field.ceiling ("\<lceil>_\<rceil>")
 
 notation Id ("skip")
      and cond_sugar ("IF _ THEN _ ELSE _" [64,64,64] 63)
-     and rtrancl ("loop")
 
 
 section\<open> Verification of regular programs \<close>
@@ -67,59 +66,63 @@ and its @{text "wp"}: @{thm fbox_cond[no_vars]}. \<close>
 
 text\<open> We also deal with finite iteration. \<close>
 
-lemma (in antidomain_kleene_algebra) fbox_starI: 
+context antidomain_kleene_algebra
+begin
+
+lemma plus_inv: "i \<le> |x] i \<Longrightarrow> j \<le> |x] j \<Longrightarrow> (i + j) \<le> |x] (i + j)"
+  by (metis ads_d_def dka.dsr5 fbox_simp fbox_subdist join.sup_mono order_trans)
+
+lemma mult_inv: "d i \<le> |x] d i \<Longrightarrow> d j \<le> |x] d j \<Longrightarrow> (d i \<cdot> d j) \<le> |x] (d i \<cdot> d j)"
+  using local.fbox_demodalisation3 local.fbox_frame local.fbox_simp by auto
+
+lemma fbox_stari: 
   assumes "d p \<le> d i" and "d i \<le> |x] i" and "d i \<le> d q"
   shows "d p \<le> |x\<^sup>\<star>] q"
-proof-
-  have "d i \<le> |x] (d i)"
-    using \<open>d i \<le> |x] i\<close> local.fbox_simp by auto
-  hence "|1] p \<le> |x\<^sup>\<star>] i" 
-    using \<open>d p \<le> d i\<close> by (metis (no_types) dual_order.trans 
-        fbox_one fbox_simp fbox_star_induct_var)
-  thus ?thesis 
-    using \<open>d i \<le> d q\<close> by (metis (full_types) fbox_mult 
-        fbox_one fbox_seq_var fbox_simp)
-qed
+   by (meson assms local.dual_order.trans fbox_iso fbox_star_induct_var)
 
-lemma rel_ad_mka_starI:
-  assumes "P \<subseteq> I" and "I \<subseteq> Q" and "I \<subseteq> wp R I"
-  shows "P \<subseteq> wp (loop R) Q"
-proof-
-  have "wp R I \<subseteq> Id"
-    by (simp add: rel_antidomain_kleene_algebra.a_subid rel_antidomain_kleene_algebra.fbox_def)
-  hence "P \<subseteq> Id" 
-    using assms(1,3) by blast
-  hence "rdom P = P" 
-    by (metis d_p2r p2r_surj)
-  also have "rdom P \<subseteq> wp (loop R) Q"
-    by (metis \<open>wp R I \<subseteq> Id\<close> assms d_p2r p2r_surj rel_antidomain_kleene_algebra.dka.dom_iso 
-        rel_antidomain_kleene_algebra.fbox_starI)
-  ultimately show ?thesis 
-    by blast
-qed
+definition loopi :: "'a \<Rightarrow> 'a \<Rightarrow> 'a" ("loop _ inv _ " [64,64] 63)
+  where "loop x inv i = x\<^sup>\<star>"
+
+lemma fbox_loopi: "d p \<le> d i \<Longrightarrow> d i \<le> |x] i \<Longrightarrow> d i \<le> d q \<Longrightarrow> d p \<le> |loop x inv i] q"
+  unfolding loopi_def using fbox_stari by blast
+
+end
+
+abbreviation loopi_sugar :: "'a rel \<Rightarrow> 'a pred \<Rightarrow> 'a rel" ("LOOP _ INV _ " [64,64] 63)
+  where "LOOP R INV I \<equiv> rel_antidomain_kleene_algebra.loopi R \<lceil>I\<rceil>"
+
+lemma wp_loopI: "\<lceil>P\<rceil> \<subseteq> \<lceil>I\<rceil> \<Longrightarrow> \<lceil>I\<rceil> \<subseteq> \<lceil>Q\<rceil> \<Longrightarrow> \<lceil>I\<rceil> \<subseteq> wp R \<lceil>I\<rceil> \<Longrightarrow> \<lceil>P\<rceil> \<subseteq> wp (LOOP R INV I) \<lceil>Q\<rceil>"
+  using rel_antidomain_kleene_algebra.fbox_loopi[of "\<lceil>P\<rceil>"] by auto
 
 
 section\<open> Verification of hybrid programs \<close>
 
-abbreviation g_evolution ::"(('a::banach)\<Rightarrow>'a) \<Rightarrow> 'a pred \<Rightarrow> real set \<Rightarrow> 'a set \<Rightarrow> 
-  real \<Rightarrow> 'a rel" ("(1x\<acute>=_ & _ on _ _ @ _)") 
-  where "(x\<acute>=f & G on T S @ t\<^sub>0) \<equiv> {(s,s') |s s'. s' \<in> g_orbital f G T S t\<^sub>0 s}"
+
+subsection \<open>Verification by providing evolution\<close>
+
+definition g_evol :: "(real \<Rightarrow> 'a \<Rightarrow> 'a) \<Rightarrow> 'a pred \<Rightarrow> real set \<Rightarrow> 'a rel" ("EVOL")
+  where "EVOL \<phi> G T = {(s,s') |s s'. s' \<in> g_orbit (\<lambda>t. \<phi> t s) G T}"
+
+lemma wp_g_dyn[simp]: "wp (EVOL \<phi> G T) \<lceil>Q\<rceil> = \<lceil>\<lambda>s. \<forall>t\<in>T. (\<forall>\<tau>\<in>down T t. G (\<phi> \<tau> s)) \<longrightarrow> Q (\<phi> t s)\<rceil>"
+  unfolding wp_rel g_evol_def g_orbit_eq by auto
 
 
 subsection \<open>Verification by providing solutions\<close>
 
-text\<open>The wlp of evolution commands. \<close>
+definition g_ode :: "(('a::banach)\<Rightarrow>'a) \<Rightarrow> 'a pred \<Rightarrow> real set \<Rightarrow> 'a set \<Rightarrow> real \<Rightarrow> 
+  'a rel" ("(1x\<acute>=_ & _ on _ _ @ _)") 
+  where "(x\<acute>= f & G on T S @ t\<^sub>0) = {(s,s') |s s'. s' \<in> g_orbital f G T S t\<^sub>0 s}"
 
-lemma wp_g_evolution: "wp (x\<acute>=f & G on T S @ t\<^sub>0) \<lceil>Q\<rceil>= 
-  \<lceil>\<lambda> s. \<forall>X\<in>ivp_sols (\<lambda>t. f) T S t\<^sub>0 s. \<forall>t\<in>T. (\<forall>\<tau>\<in>down T t. G (X \<tau>)) \<longrightarrow> Q (X t)\<rceil>"
-  unfolding g_orbital_eq wp_rel ivp_sols_def image_le_pred by auto
+lemma wp_g_orbital: "wp (x\<acute>= f & G on T S @ t\<^sub>0) \<lceil>Q\<rceil> = 
+  \<lceil>\<lambda> s. \<forall>X\<in>Sols (\<lambda>t. f) T S t\<^sub>0 s. \<forall>t\<in>T. (\<forall>\<tau>\<in>down T t. G (X \<tau>)) \<longrightarrow> Q (X t)\<rceil>"
+  unfolding g_orbital_eq wp_rel ivp_sols_def image_le_pred g_ode_def by auto
 
 context local_flow
 begin
 
-lemma wp_g_orbit: "wp (x\<acute>=f & G on T S @ 0) \<lceil>Q\<rceil> = 
+lemma wp_g_ode: "wp (x\<acute>= f & G on T S @ 0) \<lceil>Q\<rceil> = 
   \<lceil>\<lambda> s. s \<in> S \<longrightarrow> (\<forall>t\<in>T. (\<forall>\<tau>\<in>down T t. G (\<phi> \<tau> s)) \<longrightarrow> Q (\<phi> t s))\<rceil>"
-  unfolding wp_g_evolution apply(clarsimp, safe)
+  unfolding wp_g_orbital apply(clarsimp, safe)
     apply(erule_tac x="\<lambda>t. \<phi> t s" in ballE)
   using in_ivp_sols apply(force, force, force simp: init_time ivp_sols_def)
   apply(subgoal_tac "\<forall>\<tau>\<in>down T t. X \<tau> = \<phi> \<tau> s", simp_all, clarsimp)
@@ -127,27 +130,39 @@ lemma wp_g_orbit: "wp (x\<acute>=f & G on T S @ 0) \<lceil>Q\<rceil> =
   using init_time by auto
 
 lemma wp_orbit: "wp ({(s,s') | s s'. s' \<in> \<gamma>\<^sup>\<phi> s}) \<lceil>Q\<rceil> = \<lceil>\<lambda> s. s \<in> S \<longrightarrow> (\<forall> t \<in> T. Q (\<phi> t s))\<rceil>"
-  unfolding orbit_def wp_g_orbit by auto
+  unfolding orbit_def wp_g_ode g_ode_def[symmetric] by auto
 
 end
 
+
 subsection\<open> Verification with differential invariants \<close>
 
-lemma wp_g_evolution_guard: 
-  assumes "H = (\<lambda>s. G s \<and> Q s)"
-  shows "wp (x\<acute>=f & G on T S @ t\<^sub>0) \<lceil>H\<rceil> = wp (x\<acute>=f & G on T S @ t\<^sub>0) \<lceil>Q\<rceil>"
-  unfolding wp_g_evolution using assms by auto
+definition g_ode_inv :: "(('a::banach)\<Rightarrow>'a) \<Rightarrow> 'a pred \<Rightarrow> real set \<Rightarrow> 'a set \<Rightarrow> 
+  real \<Rightarrow> 'a pred \<Rightarrow> 'a rel" ("(1x\<acute>=_ & _ on _ _ @ _ DINV _ )") 
+  where "(x\<acute>= f & G on T S @ t\<^sub>0 DINV I) = (x\<acute>= f & G on T S @ t\<^sub>0)"
 
-lemma wp_g_evolution_inv:
-  assumes "\<lceil>P\<rceil> \<le> \<lceil>I\<rceil>" and "\<lceil>I\<rceil> \<le> wp (x\<acute>=f & G on T S @ t\<^sub>0) \<lceil>I\<rceil>" and "\<lceil>I\<rceil> \<le> \<lceil>Q\<rceil>"
-  shows "\<lceil>P\<rceil> \<le> wp (x\<acute>=f & G on T S @ t\<^sub>0) \<lceil>Q\<rceil>"
+lemma wp_g_orbital_guard: 
+  assumes "H = (\<lambda>s. G s \<and> Q s)"
+  shows "wp (x\<acute>= f & G on T S @ t\<^sub>0) \<lceil>Q\<rceil> = wp (x\<acute>= f & G on T S @ t\<^sub>0) \<lceil>H\<rceil>"
+  unfolding wp_g_orbital using assms by auto
+
+lemma wp_g_orbital_inv:
+  assumes "\<lceil>P\<rceil> \<le> \<lceil>I\<rceil>" and "\<lceil>I\<rceil> \<le> wp (x\<acute>= f & G on T S @ t\<^sub>0) \<lceil>I\<rceil>" and "\<lceil>I\<rceil> \<le> \<lceil>Q\<rceil>"
+  shows "\<lceil>P\<rceil> \<le> wp (x\<acute>= f & G on T S @ t\<^sub>0) \<lceil>Q\<rceil>"
   using assms(1) apply(rule order.trans)
   using assms(2) apply(rule order.trans)
   apply(rule rel_antidomain_kleene_algebra.fbox_iso)
   using assms(3) by auto
 
-lemma wp_diff_inv: "(\<lceil>I\<rceil> \<le> wp (x\<acute>=f & G on T S @ t\<^sub>0) \<lceil>I\<rceil>) = diff_invariant I f T S t\<^sub>0 G"
-  unfolding diff_invariant_eq wp_g_evolution image_le_pred by(auto simp: p2r_def)
+lemma wp_diff_inv[simp]: "(\<lceil>I\<rceil> \<le> wp (x\<acute>= f & G on T S @ t\<^sub>0) \<lceil>I\<rceil>) = diff_invariant I f T S t\<^sub>0 G"
+  unfolding diff_invariant_eq wp_g_orbital image_le_pred by(auto simp: p2r_def)
+
+lemma wp_g_odei: "\<lceil>P\<rceil> \<le> \<lceil>I\<rceil> \<Longrightarrow> \<lceil>I\<rceil> \<le> wp (x\<acute>= f & G on T S @ t\<^sub>0) \<lceil>I\<rceil> \<Longrightarrow> \<lceil>\<lambda>s. I s \<and> G s\<rceil> \<le> \<lceil>Q\<rceil> \<Longrightarrow> 
+  \<lceil>P\<rceil> \<le> wp (x\<acute>= f & G on T S @ t\<^sub>0 DINV I) \<lceil>Q\<rceil>"
+  unfolding g_ode_inv_def apply(rule_tac b="wp (x\<acute>= f & G on T S @ t\<^sub>0) \<lceil>I\<rceil>" in order.trans)
+   apply(rule_tac I="I" in wp_g_orbital_inv, simp_all)
+  apply(subst wp_g_orbital_guard, simp)
+  by (rule rel_antidomain_kleene_algebra.fbox_iso, simp)
 
 
 subsection\<open> Derivation of the rules of dL \<close>
@@ -160,45 +175,47 @@ lemma diff_solve_axiom:
   assumes "0 \<in> T" and "is_interval T" "open T"
   shows "wp (x\<acute>=(\<lambda>s. c) & G on T UNIV @ 0) \<lceil>Q\<rceil> = 
   \<lceil>\<lambda> s. \<forall>t\<in>T. (\<P> (\<lambda> t. s + t *\<^sub>R c) (down T t) \<subseteq> {s. G s}) \<longrightarrow> Q (s + t *\<^sub>R c)\<rceil>"
-  apply(subst local_flow.wp_g_orbit[where f="\<lambda>s. c" and \<phi>="(\<lambda> t x. x + t *\<^sub>R c)"])
+  apply(subst local_flow.wp_g_ode[where f="\<lambda>s. c" and \<phi>="(\<lambda> t x. x + t *\<^sub>R c)"])
   using line_is_local_flow assms unfolding image_le_pred by auto
 
 lemma diff_solve_rule:
   assumes "local_flow f T UNIV \<phi>"
     and "\<forall>s. P s \<longrightarrow> (\<forall> t\<in>T. (\<P> (\<lambda>t. \<phi> t s) (down T t) \<subseteq> {s. G s}) \<longrightarrow> Q (\<phi> t s))"
-  shows "\<lceil>P\<rceil> \<le> wp (x\<acute>=f & G on T UNIV @ 0) \<lceil>Q\<rceil>"
-  using assms by(subst local_flow.wp_g_orbit, auto)
+  shows "\<lceil>P\<rceil> \<le> wp (x\<acute>= f & G on T UNIV @ 0) \<lceil>Q\<rceil>"
+  using assms by(subst local_flow.wp_g_ode, auto)
 
-lemma diff_weak_axiom: "wp (x\<acute>=f & G on T S @ t\<^sub>0) \<lceil>Q\<rceil> = wp (x\<acute>=f & G on T S @ t\<^sub>0) \<lceil>\<lambda> s. G s \<longrightarrow> Q s\<rceil>"
-  unfolding wp_g_evolution image_def by force
+lemma diff_weak_axiom: "wp (x\<acute>= f & G on T S @ t\<^sub>0) \<lceil>Q\<rceil> = wp (x\<acute>= f & G on T S @ t\<^sub>0) \<lceil>\<lambda> s. G s \<longrightarrow> Q s\<rceil>"
+  unfolding wp_g_orbital image_def by force
 
 lemma diff_weak_rule: 
   assumes "\<lceil>G\<rceil> \<le> \<lceil>Q\<rceil>"
-  shows "\<lceil>P\<rceil> \<le> wp (x\<acute>=f & G on T S @ t\<^sub>0) \<lceil>Q\<rceil>"
+  shows "\<lceil>P\<rceil> \<le> wp (x\<acute>= f & G on T S @ t\<^sub>0) \<lceil>Q\<rceil>"
   using assms apply(subst wp_rel)
-  by(auto simp: g_orbital_eq)
+  by(auto simp: g_orbital_eq g_ode_def)
 
-lemma wp_g_orbit_IdD:
-  assumes "wp (x\<acute>=f & G on T S @ t\<^sub>0) \<lceil>C\<rceil> = Id"
-    and "\<forall>\<tau>\<in>(down T t). (s, x \<tau>) \<in> (x\<acute>=f & G on T S @ t\<^sub>0)"
+lemma wp_g_evol_IdD:
+  assumes "wp (x\<acute>= f & G on T S @ t\<^sub>0) \<lceil>C\<rceil> = Id"
+    and "\<forall>\<tau>\<in>(down T t). (s, x \<tau>) \<in> (x\<acute>= f & G on T S @ t\<^sub>0)"
   shows "\<forall>\<tau>\<in>(down T t). C (x \<tau>)"
 proof
   fix \<tau> assume "\<tau> \<in> (down T t)"
   hence "x \<tau> \<in> g_orbital f G T S t\<^sub>0 s" 
-    using assms(2) by blast
+    using assms(2) unfolding g_ode_def by blast
   also have "\<forall>y. y \<in> (g_orbital f G T S t\<^sub>0 s) \<longrightarrow> C y" 
-    using assms(1) unfolding wp_rel by(auto simp: p2r_def)
+    using assms(1) unfolding wp_rel g_ode_def by(auto simp: p2r_def)
   ultimately show "C (x \<tau>)" 
     by blast
 qed
 
 lemma diff_cut_axiom:
   assumes Thyp: "is_interval T" "t\<^sub>0 \<in> T"
-    and "wp (x\<acute>=f & G on T S @ t\<^sub>0) \<lceil>C\<rceil> = Id"
-  shows "wp (x\<acute>=f & G on T S @ t\<^sub>0) \<lceil>Q\<rceil> = wp (x\<acute>=f & (\<lambda>s. G s \<and> C s) on T S @ t\<^sub>0) \<lceil>Q\<rceil>"
-proof(rule_tac f="\<lambda> x. wp x \<lceil>Q\<rceil>" in HOL.arg_cong, clarsimp, rule subset_antisym, safe)
-  {fix s and s' assume "s' \<in> g_orbital f G T S t\<^sub>0 s"
-    then obtain \<tau>::real and X where x_ivp: "X \<in> ivp_sols (\<lambda>t. f) T S t\<^sub>0 s" 
+    and "wp (x\<acute>= f & G on T S @ t\<^sub>0) \<lceil>C\<rceil> = Id"
+  shows "wp (x\<acute>= f & G on T S @ t\<^sub>0) \<lceil>Q\<rceil> = wp (x\<acute>= f & (\<lambda>s. G s \<and> C s) on T S @ t\<^sub>0) \<lceil>Q\<rceil>"
+proof(rule_tac f="\<lambda> x. wp x \<lceil>Q\<rceil>" in HOL.arg_cong, rule subset_antisym)
+  show "(x\<acute>=f & G on T S @ t\<^sub>0) \<subseteq> (x\<acute>=f & \<lambda>s. G s \<and> C s on T S @ t\<^sub>0)"
+  proof(clarsimp simp: g_ode_def)
+    fix s and s' assume "s' \<in> g_orbital f G T S t\<^sub>0 s"
+    then obtain \<tau>::real and X where x_ivp: "X \<in> Sols (\<lambda>t. f) T S t\<^sub>0 s" 
       and "X \<tau> = s'" and "\<tau> \<in> T" and guard_x:"(\<P> X (down T \<tau>) \<subseteq> {s. G s})"
       using g_orbitalD[of s' "f" G T S t\<^sub>0 s] by blast
     have "\<forall>t\<in>(down T \<tau>). \<P> X (down T t) \<subseteq> {s. G s}"
@@ -208,39 +225,41 @@ proof(rule_tac f="\<lambda> x. wp x \<lceil>Q\<rceil>" in HOL.arg_cong, clarsimp
     ultimately have "\<forall>t\<in>(down T \<tau>). X t \<in> g_orbital f G T S t\<^sub>0 s"
       using g_orbitalI[OF x_ivp] by (metis (mono_tags, lifting))
     hence "\<forall>t\<in>(down T \<tau>). C (X t)" 
-      using wp_g_orbit_IdD[OF assms(3)] by blast
-    hence "s' \<in> g_orbital f (\<lambda>s. G s \<and> C s) T S t\<^sub>0 s"
+      using wp_g_evol_IdD[OF assms(3)] unfolding g_ode_def by blast
+    thus "s' \<in> g_orbital f (\<lambda>s. G s \<and> C s) T S t\<^sub>0 s"
       using g_orbitalI[OF x_ivp \<open>\<tau> \<in> T\<close>] guard_x \<open>X \<tau> = s'\<close> 
-      unfolding image_le_pred by fastforce}
-  thus "\<And>s s'. s' \<in> g_orbital f G T S t\<^sub>0 s \<Longrightarrow> s' \<in> g_orbital f (\<lambda>s. G s \<and> C s) T S t\<^sub>0 s"
-    by blast
-next show "\<And>s s'. s' \<in> g_orbital f (\<lambda>s. G s \<and> C s) T S t\<^sub>0 s \<Longrightarrow> s' \<in> g_orbital f G T S t\<^sub>0 s"  
-    by (auto simp: g_orbital_eq)
+      unfolding image_le_pred by fastforce
+  qed
+next show "(x\<acute>=f & \<lambda>s. G s \<and> C s on T S @ t\<^sub>0) \<subseteq> (x\<acute>=f & G on T S @ t\<^sub>0)"  
+    by (auto simp: g_orbital_eq g_ode_def)
 qed
 
 lemma diff_cut_rule:
   assumes Thyp: "is_interval T" "t\<^sub>0 \<in> T"
-    and wp_C: "\<lceil>P\<rceil> \<le> wp (x\<acute>=f & G on T S @ t\<^sub>0) \<lceil>C\<rceil>"
-    and wp_Q: "\<lceil>P\<rceil> \<subseteq> wp (x\<acute>=f & (\<lambda>s. G s \<and> C s) on T S @ t\<^sub>0) \<lceil>Q\<rceil>"
-  shows "\<lceil>P\<rceil> \<subseteq> wp (x\<acute>=f & G on T S @ t\<^sub>0) \<lceil>Q\<rceil>"
-proof(subst wp_rel, simp add: g_orbital_eq p2r_def image_le_pred, clarsimp)
+    and wp_C: "\<lceil>P\<rceil> \<le> wp (x\<acute>= f & G on T S @ t\<^sub>0) \<lceil>C\<rceil>"
+    and wp_Q: "\<lceil>P\<rceil> \<subseteq> wp (x\<acute>= f & (\<lambda>s. G s \<and> C s) on T S @ t\<^sub>0) \<lceil>Q\<rceil>"
+  shows "\<lceil>P\<rceil> \<subseteq> wp (x\<acute>= f & G on T S @ t\<^sub>0) \<lceil>Q\<rceil>"
+proof(subst wp_rel, simp add: g_orbital_eq p2r_def image_le_pred g_ode_def, clarsimp)
   fix t::real and X::"real \<Rightarrow> 'a" and s assume "P s" and "t \<in> T"
-    and x_ivp:"X \<in> ivp_sols (\<lambda>t. f) T S t\<^sub>0 s" 
+    and x_ivp:"X \<in> Sols (\<lambda>t. f) T S t\<^sub>0 s" 
     and guard_x:"\<forall>x. x \<in> T \<and> x \<le> t \<longrightarrow> G (X x)"
   have "\<forall>t\<in>(down T t). X t \<in> g_orbital f G T S t\<^sub>0 s"
     using g_orbitalI[OF x_ivp] guard_x unfolding image_le_pred by auto
   hence "\<forall>t\<in>(down T t). C (X t)" 
-    using wp_C \<open>P s\<close> by (subst (asm) wp_rel, auto)
+    using wp_C \<open>P s\<close> by (subst (asm) wp_rel, auto simp: g_ode_def)
   hence "X t \<in> g_orbital f (\<lambda>s. G s \<and> C s) T S t\<^sub>0 s"
     using guard_x \<open>t \<in> T\<close> by (auto intro!: g_orbitalI x_ivp)
   thus "Q (X t)"
-    using \<open>P s\<close> wp_Q by (subst (asm) wp_rel) auto
+    using \<open>P s\<close> wp_Q by (subst (asm) wp_rel) (auto simp: g_ode_def)
 qed
 
 text\<open>The rules of dL\<close>
 
-abbreviation g_evol ::"(('a::banach)\<Rightarrow>'a) \<Rightarrow> 'a pred \<Rightarrow> 'a rel" ("(1x\<acute>=_ & _)") 
-  where "(x\<acute>=f & G) \<equiv> (x\<acute>=f & G on UNIV UNIV @ 0)"
+abbreviation g_global_ode ::"(('a::banach)\<Rightarrow>'a) \<Rightarrow> 'a pred \<Rightarrow> 'a rel" ("(1x\<acute>=_ & _)") 
+  where "(x\<acute>= f & G) \<equiv> (x\<acute>= f & G on UNIV UNIV @ 0)"
+
+abbreviation g_global_ode_inv :: "(('a::banach)\<Rightarrow>'a) \<Rightarrow> 'a pred \<Rightarrow> 'a pred \<Rightarrow> 'a rel" 
+  ("(1x\<acute>=_ & _ DINV _)") where "(x\<acute>= f & G DINV I) \<equiv> (x\<acute>= f & G on UNIV UNIV @ 0 DINV I)"
 
 lemma DS: 
   fixes c::"'a::{heine_borel, banach}"
@@ -250,33 +269,33 @@ lemma DS:
 lemma solve:
   assumes "local_flow f UNIV UNIV \<phi>"
     and "\<forall>s. P s \<longrightarrow> (\<forall>t. (\<forall>\<tau>\<le>t. G (\<phi> \<tau> s)) \<longrightarrow> Q (\<phi> t s))"
-  shows "\<lceil>P\<rceil> \<le> wp (x\<acute>=f & G) \<lceil>Q\<rceil>"
+  shows "\<lceil>P\<rceil> \<le> wp (x\<acute>= f & G) \<lceil>Q\<rceil>"
   apply(rule diff_solve_rule[OF assms(1)])
   using assms(2) unfolding image_le_pred by simp
 
-lemma DW: "wp (x\<acute>=f & G) \<lceil>Q\<rceil> = wp (x\<acute>=f & G) \<lceil>\<lambda>s. G s \<longrightarrow> Q s\<rceil>"
+lemma DW: "wp (x\<acute>= f & G) \<lceil>Q\<rceil> = wp (x\<acute>= f & G) \<lceil>\<lambda>s. G s \<longrightarrow> Q s\<rceil>"
   by (rule diff_weak_axiom)
   
-lemma dW: "\<lceil>G\<rceil> \<le> \<lceil>Q\<rceil> \<Longrightarrow> \<lceil>P\<rceil> \<le> wp (x\<acute>=f & G) \<lceil>Q\<rceil>"
+lemma dW: "\<lceil>G\<rceil> \<le> \<lceil>Q\<rceil> \<Longrightarrow> \<lceil>P\<rceil> \<le> wp (x\<acute>= f & G) \<lceil>Q\<rceil>"
   by (rule diff_weak_rule)
 
 lemma DC:
-  assumes "wp (x\<acute>=f & G) \<lceil>C\<rceil> = Id"
-  shows "wp (x\<acute>=f & G) \<lceil>Q\<rceil> = wp (x\<acute>=f & (\<lambda>s. G s \<and> C s)) \<lceil>Q\<rceil>"
+  assumes "wp (x\<acute>= f & G) \<lceil>C\<rceil> = Id"
+  shows "wp (x\<acute>= f & G) \<lceil>Q\<rceil> = wp (x\<acute>= f & (\<lambda>s. G s \<and> C s)) \<lceil>Q\<rceil>"
   apply (rule diff_cut_axiom) 
   using assms by auto
 
 lemma dC:
-  assumes "\<lceil>P\<rceil> \<le> wp (x\<acute>=f & G) \<lceil>C\<rceil>"
-    and "\<lceil>P\<rceil> \<le> wp (x\<acute>=f & (\<lambda>s. G s \<and> C s)) \<lceil>Q\<rceil>"
-  shows "\<lceil>P\<rceil> \<le> wp (x\<acute>=f & G) \<lceil>Q\<rceil>"
+  assumes "\<lceil>P\<rceil> \<le> wp (x\<acute>= f & G) \<lceil>C\<rceil>"
+    and "\<lceil>P\<rceil> \<le> wp (x\<acute>= f & (\<lambda>s. G s \<and> C s)) \<lceil>Q\<rceil>"
+  shows "\<lceil>P\<rceil> \<le> wp (x\<acute>= f & G) \<lceil>Q\<rceil>"
   apply(rule diff_cut_rule)
   using assms by auto
 
 lemma dI:
   assumes "\<lceil>P\<rceil> \<le> \<lceil>I\<rceil>" and "diff_invariant I f UNIV UNIV 0 G" and "\<lceil>I\<rceil> \<le> \<lceil>Q\<rceil>"
-  shows "\<lceil>P\<rceil> \<le> wp (x\<acute>=f & G) \<lceil>Q\<rceil>"
-  apply(rule wp_g_evolution_inv[OF assms(1) _ assms(3)])
+  shows "\<lceil>P\<rceil> \<le> wp (x\<acute>= f & G) \<lceil>Q\<rceil>"
+  apply(rule wp_g_orbital_inv[OF assms(1) _ assms(3)])
   unfolding wp_diff_inv using assms(2) .
 
 end
